Update

Auto/Embedding/LamBase.lean
@@ -1536,47 +1536,6 @@ def LamWF.ofLamCheck? {ltv : LamTyVal} :
   | .some (LamSort.base _), _ => intro contra; cases contra
   | .none, _ => intro contra; cases contra
 
--- Interpreting while typechecking a `λ` term. If the term fails to
---   typecheck at some point, return `⟨.base .prop, GLift.up False⟩`
---   as a default value.
-def LamTerm.interp.{u} (lval : LamValuation.{u}) (lctxTy : Nat → LamSort) :
-  (t : LamTerm) → (s : LamSort) ×
-    ((lctxTerm : ∀ n, (lctxTy n).interp lval.tyVal) → s.interp lval.tyVal)
-| .atom n => ⟨lval.lamVarTy n, fun _ => lval.varVal n⟩
-| .etom n => ⟨lval.lamEVarTy n, fun _ => lval.eVarVal n⟩
-| .base b =>
-  ⟨b.lamCheck lval.toLamTyVal,
-    fun _ => LamBaseTerm.interp lval b⟩
-| .bvar n => ⟨lctxTy n, fun lctxTerm => lctxTerm n⟩
-| .lam s body =>
-  match LamTerm.interp lval (pushLCtx s lctxTy) body with
-  | ⟨bodyTy, bodyInterp⟩ =>
-    ⟨.func s bodyTy, fun lctxTerm (x : s.interp lval.tyVal) =>
-      bodyInterp (pushLCtxDep (rty:=lctxTy) x lctxTerm)⟩
-| .app s fn arg =>
-  match LamTerm.interp lval lctxTy fn with
-  | ⟨fnTy, fnInterp⟩ =>
-    match LamTerm.interp lval lctxTy arg with
-    | ⟨argTy, argInterp⟩ =>
-      match fnTy with
-      | .atom _ => ⟨.base .prop, fun _ => GLift.up False⟩
-      | .base _ => ⟨.base .prop, fun _ => GLift.up False⟩
-      | .func argTy' resTy =>
-        match heq : LamSort.beq argTy' argTy, heqa : LamSort.beq argTy' s with
-        | true, true =>
-          have heq' := LamSort.eq_of_beq_eq_true heq;
-          ⟨resTy, fun lctxTerm => (fnInterp lctxTerm) (heq' ▸ argInterp lctxTerm)⟩
-        | true,  false => ⟨.base .prop, fun _ => GLift.up False⟩
-        | false, true  => ⟨.base .prop, fun _ => GLift.up False⟩
-        | false, false => ⟨.base .prop, fun _ => GLift.up False⟩
-
-def LamTerm.interpAsProp.{u}
-  (lval : LamValuation.{u}) (lctxTy : Nat → LamSort)
-  (lctxTerm : ∀ n, (lctxTy n).interp lval.tyVal) (t : LamTerm) : GLift.{1, u} Prop :=
-  match t.interp lval lctxTy with
-  | ⟨.base .prop, tInterp⟩ => tInterp lctxTerm
-  | _ => GLift.up False
-
 def LamWF.interp.{u} (lval : LamValuation.{u}) :
   (lctxTy : Nat → LamSort) → (lctxTerm : ∀ n, (lctxTy n).interp lval.tyVal) →
   (lwf : LamWF lval.toLamTyVal ⟨lctxTy, t, rty⟩) → rty.interp lval.tyVal
@@ -1617,39 +1576,6 @@ theorem LamWF.interp_heq (lval : LamValuation.{u})
   have HUniq := LamWF.unique lwf₁ lwf₂
   cases HUniq; case intro left right =>
     cases left; cases right; rfl
-
-theorem LamTerm.interp_equiv
-  (lval : LamValuation.{u}) (lctxTy : Nat → LamSort) (lwf : LamWF lval.toLamTyVal ⟨lctxTy, t, rty⟩) :
-  ⟨rty, fun lctxTerm => LamWF.interp lval lctxTy lctxTerm lwf⟩ = LamTerm.interp lval lctxTy t := by
-  induction t generalizing lctxTy rty <;> try (cases lwf; rfl)
-  case base b =>
-    let .ofBase bH := lwf; apply eq_sigma_of_heq
-    case h₁ => rw [LamBaseTerm.lamCheck_of_LamWF bH]
-    case h₂ =>
-      apply HEq.funext; intros _; apply LamBaseTerm.interp_equiv
-  case lam s t IH =>
-    let .ofLam bodyTy H := lwf; apply eq_sigma_of_heq
-    case h₁ => rw [← IH _ H]
-    case h₂ =>
-      dsimp [LamWF.interp, interp];
-      apply HEq.funext; intros lctxTerm
-      apply HEq.funext; intros x
-      rw [← IH _ H]
-  case app s fn arg IHFn IHArg =>
-    let .ofApp _ HFn HArg := lwf
-    dsimp [LamWF.interp, interp]
-    have IHFn' := heq_of_eq_sigma (IHFn _ HFn)
-    have IHArg' := heq_of_eq_sigma (IHArg _ HArg)
-    revert IHFn' IHArg'
-    match LamTerm.interp lval lctxTy fn with
-    | ⟨fnTy, fnInterp⟩ =>
-      match LamTerm.interp lval lctxTy arg with
-      | ⟨argTy, argInterp⟩ =>
-        dsimp; intros IHFn' IHArg'
-        let ⟨fnTyEq, fnInterpEq⟩ := IHFn'
-        let ⟨argTyEq, argInterpEq⟩ := IHArg'
-        cases fnTyEq; cases argTyEq; cases fnInterpEq; cases argInterpEq
-        dsimp; rw [LamSort.beq_refl]
 
 -- In most use cases, we would have `b = .prop`
 theorem LamWF.interp_substLCtxTerm
@@ -2294,15 +2220,6 @@ def LamNonempty (tyVal : Nat → Type u) (s : LamSort) := Nonempty (s.interp tyV
 @[reducible] def dfLCtxTerm (val : Nat → Type u) : ∀ n, LamSort.interp val (dfLCtxTy n) :=
   fun _ => GLift.up.{1, u} False
 
-theorem LamThmValid.getDefault (H : LamThmValid lval [] t) :
-  GLift.down (LamTerm.interpAsProp lval dfLCtxTy (dfLCtxTerm lval.tyVal) t) := by
-  have ⟨wf, H⟩ := H dfLCtxTy
-  have hTermEquiv := LamTerm.interp_equiv _ dfLCtxTy wf
-  dsimp [LamTerm.interpAsProp]; rw [← hTermEquiv]; apply H
-
-theorem LamThmValid.getFalse (H : LamThmValid lval [] (.base .falseE)) : False :=
-  LamThmValid.getDefault H
-
 theorem LamThmWFP.ofLamThmWF (H : LamThmWF lval lctx s t) :
   LamThmWFP lval lctx s t :=
   fun lctx => Nonempty.intro (H lctx)
@@ -2527,24 +2444,6 @@ theorem LamValid.prepend (H : LamValid lval lctx t)
 theorem LamThmValid.prepend (H : LamThmValid lval lctx t)
   (ex : List LamSort) : LamThmValid lval (ex ++ lctx) (t.bvarLifts ex.length) :=
   fun lctx' => pushLCtxs_append _ _ _ ▸ LamValid.prepend (H lctx') ex
-
--- Only accepts propositions `p` without loose bound variables
-theorem LamThmValid.ofInterpAsProp
-  (lval : LamValuation) (p : LamTerm)
-  (h₁ : LamTerm.lamCheck? lval.toLamTyVal dfLCtxTy p = .some (.base .prop))
-  (h₂ : (LamTerm.interpAsProp lval dfLCtxTy (dfLCtxTerm _) p).down)
-  (h₃ : p.maxLooseBVarSucc = 0) : LamThmValid lval [] p := by
-  intros lctx';
-  have h₁' := Eq.trans (LamTerm.lamCheck?_irrelevence (lctx₁:=lctx') (by
-    intro n hlt; rw [h₃] at hlt; cases hlt)) h₁
-  have wf₁ := LamWF.ofLamCheck? h₁'; exists wf₁; intros lctxTerm
-  have wf₂ := LamWF.ofLamCheck? h₁
-  have hieq := LamTerm.interp_equiv _ _ wf₂
-  dsimp [LamTerm.interpAsProp] at h₂; rw [← hieq] at h₂; dsimp at h₂
-  apply Eq.mp _ h₂
-  apply congrArg; apply eq_of_heq;
-  apply LamWF.interp_lctxIrrelevance (lctxTy₁:=dfLCtxTy) (lctxTerm₁:=dfLCtxTerm _) _ _
-  intros n h; rw [h₃] at h; cases h
 
 theorem LamThmWF.maxLooseBVarSucc (H : LamThmWF lval lctx rty t) :
   t.maxLooseBVarSucc ≤ lctx.length := by
